\documentclass[11pt]{article}
\begin{document}
6(a).

\underline{\textbf{Given:}}
\begin{itemize}
	\item $tf'_{ij} = tf'_{ij} * (1+ \sum_0^j \frac{p_{ij}logp_{ij}}{logm})$ where $p_{ij} = \frac{tf_{ij}}{gf_i}$
	\item $0< tf_{ij} <=k $
	\item $gf_i = \sum_1^m tf_{ij}$ \\-above represents the number of times 
	ith term appears in all documents
	\item $1<m$ \\-above represents max number of documents
\end{itemize}


\vspace{5mm}
\underline{\textbf{Proof:}}

\textbf{Min:} 

-Occurs when $tf_{ij} =1$ (aka only 1 of ith term found in each document)

\vspace{5mm}
\underline{Step 1:} Assume $tf_{ij} =1$ and solve for $p_{ij}$ 

$p_{ij} = \frac{tf_{ij}}{\sum_1^m tf_{ij}} = \frac{1}{\sum_1^m 1} = \frac {1}{m}$

\vspace{5mm}
\underline{Step 2:} plug in the values for $p_{ij}$ and $tf_{ij}$ into the $tf'_{ij}$ formula
 
 $tf'_{ij} = tf_{ij} * (1+ \sum_0^j \frac{p_{ij}logp_{ij}}{logm})$
 
 \qquad $ = 1 * (1 + \sum_0^j \frac{\frac{1}{m}log\frac{1}{m}}{logm})$
 
 \qquad $ = 1+ j[\frac{\frac{1}{m}log\frac{1}{m}}{logm}]$
 
 \qquad $= 1 + \frac{-j}{m}$
 
 \qquad $=\frac{m-j}{m}$
 
 \vspace{5mm}
 \textbf{Ans:} $=\frac{m-j}{m}$
 
\vspace{5mm}
\textbf{Max:}

-Occurs when $tf_{ij} =k$ (aka only k(max frequency) of ith term is found in each document)

\vspace{5mm}
\underline{Step 1:} Assume $tf_{ij} =k$ and solve for $p_{ij}$ 

$p_{ij} = \frac{tf_{ij}}{\sum_1^m tf_{ij}} = \frac{k}{\sum_1^m k} = \frac {k}{km} = \frac{1}{m}$

\vspace{25mm}
\underline{Step 2:} plug in the values for $p_{ij}$ and $tf_{ij}$ into the $tf'_{ij}$ formula
 
 $tf'_{ij} = tf_{ij} * (1+ \sum_0^j \frac{p_{ij}logp_{ij}}{logm})$
 
 \qquad $ = k * (1 + \sum_0^j \frac{\frac{1}{m}log\frac{1}{m}}{logm})$
 
 \qquad $ = k * (1 + \frac{-j}{m})$
 
 \qquad $= \frac{k(m-j)}{m}$
 
 \vspace{5mm}
 \textbf{Ans:} $= \frac{k(m-j)}{m}$
 
 \vspace{15mm}
 b.)
\textbf{Ans: The purpose of this transformation is to get the average occurrence of the ith term found from the first to the jth document.}
\end{document}